src/extensions/paths/PreciseTyping.v
@@ -11,691 +11,26 @@ Set Implicit Arguments.
 Require Import Sequences.
 Require Import Coq.Program.Equality List.
 Require Import Definitions Binding RecordAndInertTypes Subenvironments Narrowing.
-
-Definition is_sngl T := exists p, T = typ_sngl p.
-Definition inert_sngl T := inert_typ T \/ is_sngl T.
-
-Ltac invert_repl :=
-  repeat match goal with
-         | [H: repl_dec _ _ _ {_ ⦂ _} _ |- _ ] =>
-           inversions H
-         | [H: repl_dec _ _ _ _ {_ ⦂ _} |- _ ] =>
-           inversions H
-         | [H: repl_dec _ _ _ {_ >: _ <: _} _ |- _ ] =>
-           inversions H
-         | [H: repl_dec _ _ _ _ {_ >: _ <: _} |- _ ] =>
-           inversions H
-         | [H: repl_typ _ _ _ (typ_rcd _) _ |- _ ] =>
-           inversions H
-         | [H: repl_typ _ _ _ _ (typ_rcd _) |- _ ] =>
-           inversions H
-         | [H: repl_typ _ _ _ (typ_and _ _) _ |- _ ] =>
-           inversions H
-         | [H: repl_typ _ _ _ _ (typ_and _ _) |- _ ] =>
-           inversions H
-         | [H: repl_typ _ _ _ (typ_bnd _) _ |- _ ] =>
-           inversions H
-         | [H: repl_typ _ _ _ _ (typ_bnd _) |- _ ] =>
-           inversions H
-         | [H: repl_typ _ _ _ (typ_all _ _) _ |- _ ] =>
-           inversions H
-         | [H: repl_typ _ _ _ _ (typ_all _ _) |- _ ] =>
-           inversions H
-         | [H: repl_typ _ _ _ (typ_path _ _) _ |- _ ] =>
-           inversions H
-         | [H: repl_typ _ _ _ _ (typ_path _ _) |- _ ] =>
-           inversions H
-         | [H: repl_typ _ _ _ typ_top _ |- _ ] =>
-           inversions H
-         | [H: repl_typ _ _ _ _ typ_top |- _ ] =>
-           inversions H
-         | [H: repl_typ _ _ _ typ_bot _ |- _ ] =>
-           inversions H
-         | [H: repl_typ _ _ _ _ typ_bot |- _ ] =>
-           inversions H
-         | [H: repl_typ _ _ _ (typ_sngl _) _ |- _ ] =>
-           inversions H
-         | [H: repl_typ _ _ _ _ (typ_sngl _) |- _ ] =>
-           inversions H
-    end.
-
-(* todo consistent lemma naming *)
-(* todo finish doc *)
-(** ** Precise typing *)
-(** Precise typing is used to reason about the types of paths and values.
-    Precise typing does not "modify" a path's or value's type through subtyping.
-    - For values, precise typing allows to only retrieve the "immediate" type of the value.
-      It types objects with recursive types, and functions with dependent-function types. #<br>#
-      For example, if a value is the object [nu(x: {a: T}){a = x.a}], the only way to type
-      the object through precise typing is [G ⊢! nu(x: {a: T}){a = x.a}: mu(x: {a: T})].
-    - For paths, we start out with a type [T=G(x)] (the type to which the variable is
-      bound in [G]). Then we use precise typing to additionally deconstruct [T]
-      by using recursion elimination and intersection elimination. #<br>#
-      For example, if [G(x)=mu(x: {a: T} /\ {B: S..U})], then we can derive the following
-      precise types for [x]:               #<br>#
-      [G ⊢! p: mu(x: {a: T} /\ {B: S..U})] #<br>#
-      [G ⊢! p: {a: T} /\ {B: S..U}]        #<br>#
-      [G ⊢! p: {a: T}]                    #<br>#
-      [G ⊢! p: {B: S..U}].                *)
-
-(** ** Precise typing for values *)
-Reserved Notation "G '⊢!v' v ':' T" (at level 40, v at level 59).
-
-Inductive ty_val_p : ctx -> val -> typ -> Prop :=
-
-(** [G, x: T ⊢ t^x: U^x]       #<br>#
-    [x fresh]                  #<br>#
-    [――――――――――――――――――――――――] #<br>#
-    [G ⊢! lambda(T)t: forall(T) U]     *)
-| ty_all_intro_p : forall L G T t U,
-    (forall x, x \notin L ->
-      G & x ~ T ⊢ open_trm x t : open_typ x U) ->
-    G ⊢!v val_lambda T t : typ_all T U
-
-(** [x; []; P; G, x: T^x ⊢ ds^x: T^x]       #<br>#
-    [x fresh]                               #<br>#
-    [―――――――――――――――――――――――――――――――]       #<br>#
-    [G ⊢! ν(T)ds: μ(T)]                     *)
-| ty_new_intro_p
-     : forall (L : fset var) (G : env typ) (T : typ) (ds : defs) (P : paths),
-       (forall x : var, x \notin L -> x; nil; P; G & x ~ open_typ x T ⊢ open_defs x ds :: open_typ x T) ->
-       G ⊢!v val_new T ds : typ_bnd T
-
-where "G '⊢!v' v ':' T" := (ty_val_p G v T).
-
-Hint Constructors ty_val_p.
-
-
-(** * Precise Flow *)
-(** We use the precise flow relation to reason about the relations between
-    the precise type of a path [G |-! p: T] and the type that the variable
-    is bound to in the context [G(x)=T'].#<br>#
-    If [G(x) = T], the [precise_flow] relation describes all the types [U] that [x] can
-    derive through precise typing ([|-!], see [ty_trm_p]).
-    If [precise_flow x G T U], then [G(x) = T] and [G |-! x: U].   #<br>#
-    For example, if [G(x) = mu(x: {a: T} /\ {B: S..U})], then we can derive the following
-    precise flows for [x]:                                                 #<br>#
-    [G ⊢! p: mu(x: {a: T} /\ {B: S..U}) ⪼ mu(x: {a: T} /\ {B: S..U}]         #<br>#
-    [G ⊢! p: mu(x: {a: T} /\ {B: S..U}) ⪼ {a: T} /\ {B: S..U}]               #<br>#
-    [G ⊢! p: mu(x: {a: T} /\ {B: S..U}) ⪼ {a: T}]                           #<br>#
-    [G ⊢! p: mu(x: {a: T} /\ {B: S..U}) ⪼ {B: S..U}]. *)
-
-Reserved Notation "G '⊢!' p ':' T '⪼' U" (at level 40, p at level 59).
-Reserved Notation "G '⊢!!' p ':' T" (at level 40, p at level 59).
-Reserved Notation "G '⊢!!!' p ':' T" (at level 40, p at level 59).
-
-Inductive precise_flow : ctx -> path -> typ -> typ -> Prop :=
-
-(** [G(x) = T]       #<br>#
-    [ok G]           #<br>#
-    [――――――――――――――] #<br>#
-    [G ⊢! x: T ⪼ T] *)
-| pf_bind : forall x G T,
-      ok G ->
-      binds x T G ->
-      G ⊢! pvar x: T ⪼ T
-
-(** [G ⊢! p: T ⪼ {a: U}]   #<br>#
-    [――――――――――――――――――――]   #<br>#
-    [G ⊢! p.a: U ⪼ U]        *)
-  | pf_fld : forall G p a T U,
-      G ⊢! p: T ⪼ typ_rcd {a ⦂ U} ->
-      G ⊢! p•a : U ⪼ U
-
-(** [G ⊢! p: T ⪼ mu(U)] #<br>#
-    [――――――――――――――――――] #<br>#
-    [G ⊢! p: T ⪼ U^x]       *)
-  | pf_open : forall p G T U,
-      G ⊢! p: T ⪼ typ_bnd U ->
-      G ⊢! p: T ⪼ open_typ_p p U
-
-(** [G ⊢! p: T ⪼ U1 /\ U2]   #<br>#
-    [――――――――――――――――――――]   #<br>#
-    [G ⊢! p: T ⪼ U1]        *)
-  | pf_and1 : forall p G T U1 U2,
-      G ⊢! p: T ⪼ typ_and U1 U2 ->
-      G ⊢! p: T ⪼ U1
-
-(** [G ⊢! p: T ⪼ U1 /\ U2]   #<br>#
-    [――――――――――――――――――――]   #<br>#
-    [G ⊢! p: T ⪼ U2]        *)
-  | pf_and2 : forall p G T U1 U2,
-      G ⊢! p: T ⪼ typ_and U1 U2 ->
-      G ⊢! p: T ⪼ U2
-
-where "G '⊢!' p ':' T '⪼' U" := (precise_flow G p T U).
-
-Hint Constructors precise_flow.
-
-Ltac fresh_constructor_p :=
-  apply_fresh ty_new_intro_p as z ||
-  apply_fresh ty_all_intro_p as z; auto.
-
-Lemma precise_to_general_h: forall G p T U,
-    G ⊢! p : T ⪼ U ->
-    G ⊢ trm_path p: T /\ G ⊢ trm_path p: U.
-Proof.
-  intros. induction H; intros; subst; destruct_all; eauto.
-  split; constructor*.
-Qed.
-
-(** Precise typing implies general typing. *)
-(** - for variables *)
-Lemma precise_to_general: forall G p T U,
-    G ⊢! p : T ⪼ U->
-    G ⊢ trm_path p: U.
-Proof.
-  apply* precise_to_general_h.
-Qed.
-
-(** - for values *)
-Lemma precise_to_general_v: forall G v T,
-    G ⊢!v v : T ->
-    G ⊢ trm_val v: T.
-Proof.
-  intros. induction H; intros; subst; eauto.
-Qed.
-
-Lemma narrow_to_precise_v : forall G G' v T,
-    G ⊢!v v: T ->
-    G' ⪯ G ->
-    G' ⊢!v v: T.
-Proof.
-  introv Hv Hs. inversions Hv; fresh_constructor_p;
-  assert (z \notin L) as Hz by auto; specialize (H z Hz);
-  (apply* narrow_typing || apply* narrow_defs); destruct (subenv_implies_ok Hs);
-  apply* subenv_extend; apply ok_push.
-Qed.
-
-(** ** Precise Flow Lemmas *)
-
-Lemma pf_U_top: forall p G T,
-    G ⊢! p: typ_top ⪼ T ->
-    T = typ_top.
-Proof.
-  introv Pf.
-  dependent induction Pf; auto;
-    try (specialize (IHPf eq_refl); inversion IHPf).
-Qed.
-
-(** The following two lemmas say that the type to which a variable is bound in an inert context is inert. *)
-Lemma binds_inert : forall G x T,
-    binds x T G ->
-    inert G ->
-    inert_typ T.
-Proof.
-  introv Bi Hinert. induction Hinert.
-  - false * binds_empty_inv.
-  - destruct (binds_push_inv Bi).
-    + destruct H1. subst. assumption.
-    + destruct H1. apply (IHHinert H2).
-Qed.
-
-Lemma pf_TT: forall G p T U,
-    G ⊢! p: T ⪼ U ->
-    G ⊢! p: T ⪼ T.
-Proof.
-  introv Hp. induction Hp; eauto.
-Qed.
-
-(** The precise type of a value is inert. *)
-Lemma pfv_inert : forall G v T,
-    G ⊢!v v : T ->
-    inert_typ T.
-Proof.
-  introv Ht. inversions Ht. econstructor; rename T0 into T.
-  pick_fresh z. assert (Hz: z \notin L) by auto.
-  match goal with
-  | [H: forall x, _ \notin _ -> _ |- _ ] =>
-    specialize (H z Hz);
-      pose proof (ty_defs_record_type H) as Hr;
-      destruct Hr as [ls Hr];
-      apply inert_typ_bnd with ls;
-      destruct_notin;
-      apply* record_open
-  end.
-Qed.
-
-Lemma pf_forall_U : forall G p T U S,
-    G ⊢! p: typ_all T U ⪼ S ->
-    S = typ_all T U.
-Proof.
-  introv Pf. dependent induction Pf; eauto;
-               try (repeat specialize (IHPf _ _ eq_refl); destruct_all; inversion IHPf);
-               try (specialize (IHPf _ _ eq_refl); destruct_all; inversion H).
-Qed.
-
-(** See [binds_inert]. *)
-Lemma pf_inertsngl : forall G p T U,
-    inert G ->
-    G ⊢! p: T ⪼ U ->
-    inert_sngl T /\ (inert_sngl U \/ record_type U).
-Proof.
-  introv Hi Pf. induction Pf; eauto; unfolds inert_sngl.
-  - apply (binds_inert H0) in Hi. split; left*.
-  - specialize (IHPf Hi). destruct IHPf as [HT [Hd | Hd]].
-    * destruct_all; inversion H.
-      inversions H1. inversions H. inversions H1.
-    * destruct HT as [HT | HT]; split; inversions Hd; inversions H; inversions H1;
-        try solve [left*; right*; eexists; auto];
-        right*; eexists; auto.
-  - split*. destruct (IHPf Hi) as [HT [Hd | Hd]]. destruct_all; try solve [inversion H].
-    right. inversions H. eexists. apply* open_record_typ_p.
-    subst. right. inversions H. eexists. apply* open_record_typ_p. inversion H. inversion H1.
-    inversion H. inversion H1. inversion Hd. inversion H.
-  - split*. destruct (IHPf Hi) as [HT [Hd | Hd]]; destruct_all; try solve [inversions H; inversion H1];
-    inversions Hd; inversions H0; right*.
-  - split*. destruct (IHPf Hi) as [HT [Hd | Hd]]; destruct_all; try solve [inversions H; inversion H1];
-              inversions Hd; inversions H0; right*.
-Qed.
-
-(** See [binds_inert]. *)
-Lemma pf_inert : forall G p T U,
-    inert G ->
-    G ⊢! p: T ⪼ U ->
-    inert_sngl T.
-Proof.
-  introv Hi Hp. dependent induction Hp; eauto. apply (binds_inert H0) in Hi. left*.
-  apply* pf_inertsngl.
-Qed.
-
-Hint Resolve pf_inert.
-
-(** See [inert_typ_bnd_record] *)
-Lemma pf_rcd_T : forall G p T U,
-    inert G ->
-    G ⊢! p: typ_bnd T ⪼ U ->
-    record_type T.
-Proof.
-  introv Hi Pf. apply pf_inert in Pf; inversions Pf; eauto. inversion* H. destruct_all. inversions H.
-  inversion H0.
-Qed.
-
-(** If [G(x) = mu(x: T)], then [x]'s precise type can be only [mu(x: T)]
-     or a record type. *)
-Lemma pf_rec_rcd_U : forall G p T U,
-    inert G ->
-    G ⊢! p: typ_bnd T ⪼ U->
-    U = typ_bnd T \/ record_type U.
-Proof.
-  introv Hi Pf.
-  dependent induction Pf; try solve [left*].
-  - specialize (IHPf T Hi eq_refl). destruct IHPf as [eq | r].
-    * inversions eq. right. lets Hr: (pf_rcd_T Hi Pf).
-      apply* open_record_type_p.
-    * inversion r. inversion H.
-  - right. destruct (IHPf T Hi eq_refl) as [F | Hr]. inversion F.
-    inversion Hr. inversions H.
-    exists ls. assumption.
-  - right. destruct (IHPf T Hi eq_refl) as [F | Hr]. inversion F.
-    inversion Hr. inversions H.
-    eexists. apply* rt_one.
-Qed.
-
-Lemma pf_sngl_U: forall G p q U,
-    G ⊢! p : typ_sngl q ⪼ U->
-    U = typ_sngl q.
-Proof.
-  introv Hp. dependent induction Hp; eauto; try (specialize (IHHp _ eq_refl); inversion IHHp).
-Qed.
-
-(** If [x]'s precise type is [mu(x: U)], then [G(x) = mu(x: U)] *)
-Lemma pf_bnd_T: forall G p T U,
-    inert G ->
-    G ⊢! p: T ⪼ typ_bnd U ->
-    T = typ_bnd U.
-Proof.
-  introv Hi Pf.
-  lets HT: (pf_inert Hi Pf).
-  inversions HT.
-  - inversions H. apply pf_forall_U in Pf. inversion Pf.
-    apply (pf_rec_rcd_U Hi) in Pf. destruct Pf. inversion* H. inversion H. inversion H1.
-  - inversions H. apply pf_sngl_U in Pf. inversion Pf.
-Qed.
-
-Lemma pf_sngl_T: forall G p q T,
-    inert G ->
-    G ⊢! p : T ⪼ typ_sngl q ->
-    T = typ_sngl q.
-Proof.
-  introv Hi Hp. dependent induction Hp; eauto.
-  destruct U; inversions x. lets H: (pf_bnd_T Hi Hp). subst.
-  apply (pf_inert Hi) in Hp. inversion* Hp. inversions H. inversion H1. destruct_all.
-  inversion H. inversion H0.
-  lets His: (pf_inertsngl Hi Hp). destruct_all; progress (repeat inversions H0); inversion H1; inversions H0.
-  inversion H3.
-  lets His: (pf_inertsngl Hi Hp). destruct_all; progress (repeat inversions H0); inversion H1; inversions H0.
-Qed.
-
-(** If [x]'s precise type is a field or type declaration, then [G(x)] is
-    a recursive type. *)
-Lemma pf_bnd_T2: forall G p T D,
-    inert G ->
-    G ⊢! p: T ⪼ typ_rcd D ->
-    exists U, T = typ_bnd U.
-Proof.
-  introv Hi Pf.
-  lets HT: (pf_inert Hi Pf).
-  inversions HT; dependent induction Pf; auto;
-    try (solve [(destruct_all; subst; inversion H) |
-                (destruct_all; subst; apply pf_sngl_U in Pf; inversion Pf)]).
-  - inversion H1.
-  - destruct U; inversions x. apply (pf_bnd_T Hi) in Pf. destruct_all; subst; eauto.
-  - inversions H. apply pf_forall_U in Pf. inversion* Pf. eauto.
-  - inversions H. apply pf_forall_U in Pf. destruct_all. inversion Pf. eauto.
-  - inversion H1. inversion H2.
-  - inversion H. inversion H0.
-  - destruct U; inversions x. apply pf_bnd_T in Pf. subst*. auto.
-  - inversions H. apply pf_sngl_U in Pf. inversion Pf.
-  - inversions H. apply pf_sngl_U in Pf. inversion Pf.
-Qed.
-
-(** If [x]'s precise type is a record type, then [G(x)] is a recursive type. *)
-Lemma pf_bnd_T3: forall G p T Ds,
-    inert G ->
-    G ⊢! p: T ⪼ Ds ->
-    record_type Ds ->
-    exists U, T = typ_bnd U.
-Proof.
-  introv Hi Pf Hr.
-  lets HT: (pf_inert Hi Pf).
-  destruct* HT.
-  inversions H.
-  apply pf_forall_U in Pf. destruct_all. subst. inversion Hr. inversion H. eauto.
-  inversions H. apply pf_sngl_U in Pf. subst. inversion Hr. inversion H.
-Qed.
-
-(** The following two lemmas express that if [x]'s precise type is a function type,
-    then [G(x)] is the same function type. *)
-Lemma pf_forall_T : forall p G S T U,
-    inert G ->
-    G ⊢! p: T ⪼ typ_all S U->
-    T = typ_all S U.
-Proof.
-  introv Hi Pf.
-  lets Hiu: (pf_inert Hi Pf).
-  inversions Hiu.
-  - inversions H. apply pf_forall_U in Pf. inversion* Pf.
-    destruct (pf_rec_rcd_U Hi Pf) as [H1 | H1]; inversions H1. inversion H.
-  - inversions H. apply pf_sngl_U in Pf. inversion Pf.
-Qed.
-
-(** If [G ⊢! x: T ⪼ U] then [G(x) = T]. *)
-(** If [G ⊢! x: T ⪼ U] then [G(x) = T]. *)
-Lemma pf_binds: forall G x T U,
-    inert G ->
-    G ⊢! pvar x: T ⪼ U ->
-    binds x T G.
-Proof.
-  introv Hi Pf. dependent induction Pf; try simpl_dot; auto.
-Qed.
-
-(** See [pf_lambda_T]. *)
-Lemma binds_forall : forall x G S T U,
-    inert G ->
-    G ⊢! pvar x : U ⪼ typ_all S T ->
-    binds x (typ_all S T) G.
-Proof. Abort. (*
-  introv Hi Htyp. lets H: (pf_forall_T Hi Htyp). subst. destruct_all; subst.
-  repeat eexists. apply* pf_binds.
-Qed.*)
-
-(** In an inert context, the precise type of a variable
-    cannot be bottom. *)
-Lemma pf_bot : forall G p T,
-    inert G ->
-    G ⊢! p: T ⪼ typ_bot ->
-    False.
-Proof.
-  introv Hi Pf.
-  lets HT: (pf_inert Hi Pf). inversions HT.
-  - inversions H. apply pf_forall_U in Pf. inversion Pf.
-    destruct (pf_rec_rcd_U Hi Pf); inversion H0; inversion H. inversion H5. inversion H7.
-  - inversions H. apply pf_sngl_U in Pf. inversion Pf.
-Qed.
-
-(** In an inert context, the precise type of
-    a variable cannot be type selection. *)
-Lemma pf_psel : forall G T p q A,
-    inert G ->
-    G ⊢! p: T ⪼ typ_path q A ->
-    False.
-Proof.
-  introv Hi Pf.
-  lets HT: (pf_inert Hi Pf). inversions HT.
-  - inversions H.
-    * apply pf_forall_U in Pf. inversion Pf.
-    * destruct (pf_rec_rcd_U Hi Pf); inversion H. inversion H1.
-  - destruct H as [r Heq]. subst. apply pf_sngl_U in Pf. inversion Pf.
-Qed.
-
-(*Definition original_path G p T U q :=
-    G ⊢! p: T ⪼ U /\
-    G ⊢! q: T ⪼ T /\
-    (p = q \/ G ⊢! p: typ_sngl q ⪼ typ_sngl q).
-
-Lemma original_path_not_opened: forall G p T U,
-    G ⊢! p: T ⪼ U ->
-    original_path G p T U p.
-Proof.
-  introv Hp. unfold original_path. split*. split.
-  apply* pf_TT. left*.
-Qed.
-
-Lemma original_path_unique: forall G p T1 T2 U1 U2 q1 q2,
-    original_path G p T1 U1 q1 ->
-    original_path G p T2 U2 q2 ->
-    q1 = q2.
-Proof.
-  introv [Hp1 [Hq1 H1]] [Hp2 [Hq2 H2]].
-Admitted.
-
-Lemma original_path_exists: forall G p T U,
-    inert G ->
-    G ⊢! p: T ⪼ U ->
-    exists q T', original_path G p T' T' q.
-Proof.
-  introv Hi Hp. induction Hp; try specialize (IHHp Hi);
-                  try solve [unfolds original_path; destruct_all;
-                             do 2 eexists; eauto; split*].
-Qed.
-*)
-(** If [G(x) = mu(T)], and [G ⊢! p: ... /\ D /\ ...], then [T^x = ... /\ D /\ ...]. *)
-Lemma pf_record_has_T : forall p G T T' D,
-    inert G ->
-    G ⊢! p: typ_bnd T ⪼ T' ->
-    record_has T' D ->
-    (*original_path G p (typ_bnd T) T' q ->
-    record_has (open_typ_p q T) D.*)
-    record_has (open_typ_p p T) D.
-Proof.
-  introv Hi Pf Hr.
-  dependent induction Pf; eauto; try solve [inversion Hr].
-  apply pf_bnd_T in Pf; auto. inversion* Pf.
-Qed.
-
-(** If [G(x) = mu(S)] and [G ⊢! p: D], where [D] is a field or type declaration,
-    then [S^x = ... /\ D /\ ...]. *)
-Lemma pf_record_has_U: forall S G p D,
-    inert G ->
-    G ⊢! p: typ_bnd S ⪼ typ_rcd D ->
-    record_has (open_typ_p p S) D.
-Proof.
-  introv Hi Pf.
-  apply* pf_record_has_T.
-Qed.
-
-(** If
-    - [G ⊢! p: mu(T) ⪼ {A: T1..T1}]
-    - [G ⊢! p: mu(T) ⪼ {A: T2..T2}]
-    then [T1 = T2]. *)
-Lemma pf_dec_typ_unique : forall G p T A T1 T2,
-    inert G ->
-    G ⊢! p: typ_bnd T ⪼ typ_rcd {A >: T1 <: T1} ->
-    G ⊢! p: typ_bnd T ⪼ typ_rcd {A >: T2 <: T2} ->
-    T1 = T2.
-Proof.
-  introv Hi Pf1 Pf2.
-  pose proof (pf_record_has_U Hi Pf1) as H1.
-  pose proof (pf_record_has_U Hi Pf2) as H2.
-  lets Hr: (pf_rcd_T Hi Pf1).
-  assert (record_type (open_typ_p p T)) as Hrt
-      by apply* open_record_type_p.
-  apply* unique_rcd_typ.
- Qed.
-
-Lemma pf_dec_fld_unique : forall G p T a U1 U2,
-    inert G ->
-    G ⊢! p: T ⪼ typ_rcd {a ⦂ U1} ->
-    G ⊢! p: T ⪼ typ_rcd {a ⦂ U2} ->
-    U1 = U2.
-Proof.
-  introv Hi Pf1 Pf2.
-  destruct (pf_bnd_T2 Hi Pf1) as [T1 He1]. subst.
-  destruct (pf_rec_rcd_U Hi Pf1) as [Ht | Ht]; inversions Ht.
-  destruct (pf_rec_rcd_U Hi Pf2) as [Ht | Ht]; inversions Ht.
-  dependent induction Pf1.
-  - lets Hb: (pf_bnd_T Hi Pf1). inversions Hb.
-    destruct U; inversions x. destruct d; inversions H2.
-    lets Hrh: (pf_record_has_U Hi Pf2).
-    inversion* Hrh.
-  - lets Hrh: (pf_record_has_U Hi Pf2).
-    assert (record_has (typ_and (typ_rcd {a ⦂ U1}) U0) {a ⦂ U1}) as Hrh' by auto.
-    lets Hrh'': (pf_record_has_T Hi Pf1 Hrh'). apply (pf_rcd_T Hi) in Pf2.
-    lets Hrt: (open_record_type_p p Pf2). apply* unique_rcd_trm.
-  - lets Hrh: (pf_record_has_U Hi Pf2).
-    assert (record_has (typ_and U3 (typ_rcd {a ⦂ U1})) {a ⦂ U1}) as Hrh' by auto.
-    lets Hrh'': (pf_record_has_T Hi Pf1 Hrh'). apply (pf_rcd_T Hi) in Pf2.
-    lets Hrt: (open_record_type_p p Pf2). apply* unique_rcd_trm.
-Qed.
-
-Lemma pf_T_unique: forall G p T1 T2 U1 U2,
-    inert G ->
-    G ⊢! p: T1 ⪼ U1 ->
-    G ⊢! p: T2 ⪼ U2 ->
-    T1 = T2.
-Proof.
-  introv Hi Hp1. gen T2 U2. induction Hp1; introv Hp2; eauto.
-  - Case "pf_bind".
-    apply (pf_binds Hi) in Hp2. eapply binds_functional. apply H0. auto.
-  - Case "pf_fld".
-    gen U T. dependent induction Hp2; introv Hp IH; try simpl_dot; eauto.
-    * rename a2 into x. rename f0 into bs. clear IHHp2.
-      destruct (pf_bnd_T2 Hi Hp) as [S Heq]. subst. lets Hr: (pf_rcd_T Hi Hp).
-      destruct (pf_bnd_T2 Hi Hp2) as [S' Heq]. subst. lets Hr': (pf_rcd_T Hi Hp2).
-      specialize (IH Hi _ _ Hp2).
-      inversions IH. lets Hrh: (pf_record_has_U Hi Hp2).
-      lets Hrh': (pf_record_has_U Hi Hp).
-      assert (record_type (open_typ_p (p_sel x bs) S')) as Hrt by apply* open_record_type_p.
-      apply* unique_rcd_trm.
-Qed.
-
-(** If a typing context is inert, then the variables in its domain are distinct. #<br>#
-    Note: [ok] is defined in [TLC.LibEnv.v]. *)
-Lemma inert_ok : forall G,
-    inert G ->
-    ok G.
-Proof.
-  intros G HG. induction G using env_ind.
-  auto.
-  inversions HG. false* empty_push_inv.
-  destruct (eq_push_inv H) as [Hx [HT HG]]. subst.
-  apply* ok_push.
-Qed.
-
-Hint Resolve inert_ok.
-
-(** If [G ⊢! p: {A: S..U}] then [S = U]. *)
-Lemma pf_dec_typ_tight : forall G p T A S U,
-    inert G ->
-    G ⊢! p: T ⪼ typ_rcd {A >: S <: U}->
-    S = U.
-Proof.
-  introv Hi Pf. destruct (pf_bnd_T2 Hi Pf) as [V H]. subst.
-  destruct (pf_rec_rcd_U Hi Pf) as [H1 | H1]; inversions H1. inversions H.
-  inversions* H1.
-Qed.
-
-(*
-Lemma narrow_precise : forall G G' x T U,
-    G ⊢! x: T ⪼ U->
-    G' ⪯ G ->
-    exists T', G' ⊢! x: T' ⪼ U.
-Proof.
-  introv Hx Hs. inversions Hx.
-  - admit.
-
-  assert (z \notin L) as Hz by auto; specialize (H z Hz);
-  (apply* narrow_typing || apply* narrow_defs); destruct (subenv_implies_ok Hs);
-  apply* subenv_extend; apply ok_push.
-Qed.
-*)
-
-Lemma pf_strengthen: forall G y V x bs T U,
-    inert (G & y ~ V) ->
-    G & y ~ V ⊢! p_sel (avar_f x) bs : T ⪼ U->
-    x <> y ->
-    G ⊢! p_sel (avar_f x) bs : T ⪼ U.
-Proof.
-  introv Hi Ht Hneq. dependent induction Ht; eauto.
-  - apply (binds_push_neq_inv H0) in Hneq. constructor*.
-  - destruct p. inversions x.
-    specialize (IHHt _ _ _ _ _ Hi JMeq_refl eq_refl Hneq).
-    lets Hf: (pf_fld IHHt). eauto.
-Qed.
-
-Lemma pf_var_sngl : forall G x p T,
-    inert G ->
-    G ⊢! pvar x : typ_sngl p ⪼ T ->
-    False.
-Proof.
-  introv Hi Hx. dependent induction Hx; eauto.
-  apply (binds_inert H0) in Hi. inversion Hi.
-  unfolds sel_fields. destruct p0. inversion x.
-Qed.
-
-Lemma pf_inert_bnd : forall G p T D,
-    inert G ->
-    G ⊢! p : T ⪼ typ_rcd D ->
-    inert_typ T.
-Proof.
-  introv Hi Hp. lets Hr: (pf_bnd_T2 Hi Hp). destruct_all.
-  subst. apply pf_rcd_T in Hp; auto. inversions Hp. apply* inert_typ_bnd.
-Qed.
-
-Lemma pf_path_sel: forall G p a T U,
-    inert G ->
-    G ⊢! p•a : T ⪼ U ->
-    exists V W, G ⊢! p: typ_bnd V ⪼ typ_rcd {a ⦂ W}.
-Proof.
-  introv Hi Hp. dependent induction Hp; try simpl_dot; eauto.
-  destruct (pf_bnd_T2 Hi Hp) as [V Heq]. subst. eauto.
-Qed.
+Require Export PreciseFlow.
 
 Inductive precise_typing2: ctx -> path -> typ -> Prop :=
-
 | pt2: forall G p T U,
     G ⊢! p : T ⪼ U ->
     G ⊢!! p: U
-
 | pt2_sngl_trans : forall G p q a U,
     G ⊢!! p : typ_sngl q ->
     G ⊢!! q•a : U ->
     G ⊢!! p•a : typ_sngl q•a
-
 where "G '⊢!!' p ':' T" := (precise_typing2 G p T).
 
 Inductive precise_typing3: ctx -> path -> typ -> Prop :=
-
 | pt3: forall G p T,
     G ⊢!! p : T ->
     G ⊢!!! p: T
-
 | pt3_sngl_trans : forall G p q T,
     G ⊢!! p : typ_sngl q ->
     G ⊢!!! q : T ->
     G ⊢!!! p : T
-
 where "G '⊢!!!' p ':' T" := (precise_typing3 G p T).
 
 Hint Constructors precise_typing2 precise_typing3.
@@ -1109,39 +444,6 @@ Proof.
   - specialize (IHHp _ Hi eq_refl). destruct IHHp as [Hq | [r [Hr1 Hr2]]]; right*.
 Qed.
 
-
-(*Lemma field_elim_rcd1: forall G p a T T',
-    inert G ->
-    G ⊢! p • a : T' ⪼ T ->
-    (inert_typ T \/ record_type T) ->
-    exists U, G ⊢! p : U ⪼ U /\ (inert_typ U \/ record_type U).
-Proof.
-  introv Hi Hp Hir. dependent induction Hp; try simpl_dot.
-  - destruct (pf_bnd_T2 Hi Hp) as [V Heq]. subst. lets Hp': (pf_TT Hp). apply pf_open in Hp'.
-    lets Hr': (pf_rcd_T Hi Hp). exists (typ_bnd V). split. apply pf_TT in Hp'. auto. left.
-    inversions Hr'. apply* inert_typ_bnd.
-  - lets Heq: (pf_bnd_T Hi Hp). subst.
-    lets Hr: (pf_rcd_T Hi Hp).
-    apply* IHHp. destruct Hir. inversions H.  destruct U; inversions H1. inversion Hr. inversion H.
-    destruct U; inversions H0. inversion Hr. inversion H.
-    left. inversions Hr. apply* inert_typ_bnd.
-  - apply* IHHp. right. destruct (pf_inertsngl Hi Hp). destruct H0. inversions H0. inversion H1.
-    inversion H1. inversion H0. auto.
-  - apply* IHHp. right. destruct (pf_inertsngl Hi Hp). destruct H0. inversions H0. inversion H1.
-    inversion H1. inversion H0. auto.
-Qed.
-
-Lemma field_elim_rcd2: forall G p a T,
-    inert G ->
-    G ⊢!! p • a : T ->
-    (inert_typ T \/ record_type T) ->
-    exists U, G ⊢!! p : U /\ (inert_typ U \/ record_type U).
-Proof.
-  introv Hi Hp Hr. dependent induction Hp.
-  - destruct (field_elim_rcd1 _ _ Hi H Hr) as [S [Hf Hir]]. eexists. eauto.
-  - destruct Hr. inversion H. inversion H. inversion H0.
-Qed.*)
-
 Lemma pt2_exists: forall G p T,
     G ⊢!!! p: T ->
     exists U, G ⊢!! p: U.
@@ -1226,13 +528,22 @@ Definition typed_repl_comp_qp G T1 T2 :=
 
 Definition repl_composition_qp G := star (typed_repl_comp_qp G).
 
-Lemma repl_comp_sngl_inv : forall G T p,
+Lemma repl_comp_sngl_inv1 : forall G T p,
     repl_composition_qp G T (typ_sngl p) ->
     exists q, T = typ_sngl q.
 Proof.
   introv Hr. dependent induction Hr; eauto.
   specialize (IHHr _ eq_refl). destruct_all. subst.
   inversions H. destruct_all. invert_repl. eexists; eauto.
+Qed.
+
+Lemma repl_comp_sngl_inv2 : forall G T p,
+    repl_composition_qp G (typ_sngl p) T ->
+    exists q, T = typ_sngl q.
+Proof.
+  introv Hr. dependent induction Hr; eauto.
+  inversions H. destruct_all. invert_repl.
+  specialize (IHHr _ eq_refl). destruct_all. eexists. eauto.
 Qed.
 
 Lemma repl_comp_and1: forall G T T' U,
@@ -1267,8 +578,6 @@ Proof.
   assert (exists r, b = typ_sngl r) as [p3 Heq] by admit. subst.
   specialize (IHHc _ _ Hi eq_refl eq_refl Hq).
   destruct H as [r1 [r2 [n [H Hr]]]]. inversions Hr.
-  rewrite proj_rewrite_mult in *. set (p_sel qx qbs) as q in *.
-  set (p_sel px pbs) as p' in *.
   lets H': (pt3 (pt2 H)).
   destruct IHHc as [Heq | Hp]; subst.
   - lets Htt: (pt3_trans_trans _ Hi H' Hq).
@@ -1288,17 +597,11 @@ Proof.
   assert (exists r, b = typ_sngl r) as [p3 Heq] by admit. subst.
   specialize (IHHc _ _ Hi eq_refl eq_refl).
   destruct H as [r1 [r2 [n [H Hr]]]]. inversions Hr.
-  rewrite proj_rewrite_mult in *. set (p_sel qx qbs) as q in *.
-  set (p_sel px pbs) as p' in *.
   lets H': (pt3 (pt2 H)).
-  assert (exists S, G ⊢!!! q •• bs : S) as [S Hqs]. {
-    eexists. apply* pt3_field_trans.
-  }
+  lets Hqs: (pt3_field_trans _ Hi H' Hq).
   destruct (IHHc _ Hqs) as [Heq | Hp]; subst.
-  - lets Htt: (pt3_trans_trans _ Hi H' Hqs).
-    right*.
-  - right.
-    destruct (sngl_typed3 Hi Hp) as [S' Hqbs].
+  - lets Htt: (pt3_trans_trans _ Hi H' Hqs). right*.
+  - right. destruct (sngl_typed3 Hi Hp) as [S' Hqbs].
     lets Htt: (pt3_trans_trans _ Hi H' Hqbs). apply* pt3_sngl_trans3.
 Qed.
 
@@ -1309,17 +612,14 @@ Lemma field_typing_comp1: forall G r q a U,
   exists T, G ⊢!!! r•a : T.
 Proof.
   introv Hi Hr Hq. gen a U. dependent induction Hr; introv Hq; eauto.
-  destruct (repl_comp_sngl_inv Hr) as [p Heq]. subst.
+  destruct (repl_comp_sngl_inv1 Hr) as [p Heq]. subst.
   destruct H as [p' [q' [n [Hp' Hr']]]].
   specialize (IHHr _ _ Hi eq_refl eq_refl _ _ Hq). destruct IHHr as [T Hpa].
   assert (G ⊢!!! p : typ_sngl r) as Hpr. {
-    clear Hq Hr. inversions Hr'. gen qx qbs a T. induction bs; introv Hpa Hq. auto.
-    simpl. repeat rewrite proj_rewrite in *.
-    destruct (pt3_backtrack _ _ Hq) as [T1 Ht1]. simpls. rewrite proj_rewrite in *.
-    constructor*.
-    simpls. repeat rewrite proj_rewrite in *.
-    simpls. rewrite proj_rewrite in *.
-    apply pt3_backtrack in Hq. destruct_all. rewrite proj_rewrite in *.
+    clear Hq Hr. inversions Hr'. gen p' a T. induction bs; introv Hpa; introv Hq.
+    repeat rewrite field_sel_nil in *. eauto.
+    destruct (pt3_backtrack _ _ Hq) as [T1 Ht1]. rewrite proj_rewrite' in *.
+    apply pt3_backtrack in Hq. destruct_all. rewrite proj_rewrite'.
     apply* pt3_field_elim_p.
   }
   apply* field_elim_q3.
@@ -1336,9 +636,9 @@ Proof.
   destruct H0 as [q' [n [Hp Hr']]].
   assert (exists q', b = typ_sngl q') as [q'' Heq] by inversion* Hr'.
   subst. specialize (IHHr _ _ Hi eq_refl eq_refl). invert_repl. apply* IHHr. clear IHHr Hr.
-  gen px pbs a U. induction bs; intros; simpls.
-  - rewrite proj_rewrite in *. apply* pt3_trans2.
-  - do 2 rewrite app_comm_cons in *. rewrite proj_rewrite_mult in *. apply* pt3_field_trans'.
+  gen q' a U. induction bs; intros; simpls.
+  - repeat rewrite field_sel_nil in *. apply* pt3_trans2.
+  - rewrite <- proj_rewrite' in *. apply* pt3_field_trans'.
 Qed.
 
 Lemma repl_composition_fld_elim: forall G p q a T,
@@ -1354,10 +654,9 @@ Proof.
     } subst.
     specialize (IHHr _ _ Hi eq_refl eq_refl).
     destruct H as [p'' [q' [n [Hpq Hr']]]]. apply star_trans with (b:=typ_sngl p' • a).
-    * apply star_one.
-      repeat eexists. apply Hpq.
-      inversions Hr'. eapply rsngl. simpl. rewrite app_comm_cons. all: auto.
-    * invert_repl. apply* IHHr. clear IHHr. simpls. rewrite app_comm_cons.
-      rewrite proj_rewrite_mult in *.
+    * apply star_one. inversions Hr'. repeat eexists. apply Hpq.
+      repeat rewrite <- proj_rewrite' in *.
+      apply* rsngl.
+    * invert_repl. apply* IHHr. clear IHHr. rewrite <- proj_rewrite' in *.
       apply* pt3_field_trans'.
 Qed.
